Weidenbach_Book/IsaSAT/IsaSAT_Mark.thy
@@ -1,0 +1,631 @@
+theory IsaSAT_Mark
+  imports
+    IsaSAT_Clauses
+    IsaSAT_Watch_List
+    IsaSAT_Trail
+begin
+
+chapter \<open>Clauses Encoded as Positions\<close>
+
+text \<open>We use represent the conflict in two data structures close to the one used by the most SAT
+solvers: We keep an array that represent the clause (for efficient iteration on the clause) and a
+``hash-table'' to efficiently test if a literal belongs to the clause.
+
+The first data structure is simply an array to represent the clause. This theory is only about
+the second data structure. We refine it from the clause (seen as a multiset) in two steps:
+  \<^enum> First, we represent the clause as a ``hash-table'', where the \<^term>\<open>i\<close>-th position indicates
+    \<^term>\<open>Some True\<close> (respectively \<^term>\<open>Some False\<close>, \<^term>\<open>None\<close>) if \<^term>\<open>Pos i\<close> is present in the
+    clause (respectively \<^term>\<open>Neg i\<close>, not at all). This allows to represent every not-tautological
+    clause whose literals fits in the underlying array.
+
+We use the first part in two different ways: once for the conflict, where we specialize it to
+include only information on the atoms and once in the marking structure.
+\<close>
+
+text \<open>This is the first level of the refinement. We tried a few different definitions (including a
+direct one, i.e., mapping a position to the inclusion in the set) but the inductive version turned out
+to the easiest one to use.
+\<close>
+
+text \<open>This is the first level of the refinement. We tried a few different definitions (including a
+direct one, i.e., mapping a position to the inclusion in the set) but the inductive version turned out
+to the easiest one to use.
+\<close>
+inductive mset_as_position :: \<open>bool option list \<Rightarrow> nat literal multiset \<Rightarrow> bool\<close> where
+empty:
+  \<open>mset_as_position (replicate n None) {#}\<close> |
+add:
+  \<open>mset_as_position xs' (add_mset L P)\<close>
+  if \<open>mset_as_position xs P\<close> and \<open>atm_of L < length xs\<close> and \<open>L \<notin># P\<close> and \<open>-L \<notin># P\<close> and
+     \<open>xs' = xs[atm_of L := Some (is_pos L)]\<close>
+
+lemma mset_as_position_distinct_mset:
+  \<open>mset_as_position xs P \<Longrightarrow> distinct_mset P\<close>
+  by (induction rule: mset_as_position.induct) auto
+
+lemma mset_as_position_atm_le_length:
+  \<open>mset_as_position xs P \<Longrightarrow> L \<in># P \<Longrightarrow> atm_of L < length xs\<close>
+  by (induction rule: mset_as_position.induct) (auto simp: nth_list_update' atm_of_eq_atm_of)
+
+lemma mset_as_position_nth:
+  \<open>mset_as_position xs P \<Longrightarrow> L \<in># P \<Longrightarrow> xs ! (atm_of L) = Some (is_pos L)\<close>
+  by (induction rule: mset_as_position.induct)
+    (auto simp: nth_list_update' atm_of_eq_atm_of dest: mset_as_position_atm_le_length)
+
+lemma mset_as_position_in_iff_nth:
+  \<open>mset_as_position xs P \<Longrightarrow> atm_of L < length xs \<Longrightarrow> L \<in># P \<longleftrightarrow> xs ! (atm_of L) = Some (is_pos L)\<close>
+  by (induction rule: mset_as_position.induct)
+    (auto simp: nth_list_update' atm_of_eq_atm_of is_pos_neg_not_is_pos
+      dest: mset_as_position_atm_le_length)
+
+lemma mset_as_position_tautology: \<open>mset_as_position xs C \<Longrightarrow> \<not>tautology C\<close>
+  by (induction rule: mset_as_position.induct) (auto simp: tautology_add_mset)
+
+lemma mset_as_position_right_unique:
+  assumes
+    map: \<open>mset_as_position xs D\<close> and
+    map': \<open>mset_as_position xs D'\<close>
+  shows \<open>D = D'\<close>
+proof (rule distinct_set_mset_eq)
+  show \<open>distinct_mset D\<close>
+    using mset_as_position_distinct_mset[OF map] .
+  show \<open>distinct_mset D'\<close>
+    using mset_as_position_distinct_mset[OF map'] .
+  show \<open>set_mset D = set_mset D'\<close>
+    using mset_as_position_in_iff_nth[OF map] mset_as_position_in_iff_nth[OF map']
+      mset_as_position_atm_le_length[OF map] mset_as_position_atm_le_length[OF map']
+    by blast
+qed
+
+lemma mset_as_position_mset_union:
+  fixes P xs
+  defines \<open>xs' \<equiv> fold (\<lambda>L xs. xs[atm_of L := Some (is_pos L)]) P xs\<close>
+  assumes
+    mset: \<open>mset_as_position xs P'\<close> and
+    atm_P_xs: \<open>\<forall>L \<in> set P. atm_of L < length xs\<close> and
+    uL_P: \<open>\<forall>L \<in> set P. -L \<notin># P'\<close> and
+    dist: \<open>distinct P\<close> and
+    tauto: \<open>\<not>tautology (mset P)\<close>
+  shows \<open>mset_as_position xs' (mset P \<union># P')\<close>
+  using atm_P_xs uL_P dist tauto unfolding xs'_def
+proof (induction P)
+  case Nil
+  show ?case using mset by auto
+next
+  case (Cons L P) note IH = this(1) and atm_P_xs = this(2) and uL_P = this(3) and dist = this(4)
+    and tauto = this(5)
+  then have mset:
+    \<open>mset_as_position (fold (\<lambda>L xs. xs[atm_of L := Some (is_pos L)]) P xs) (mset P \<union># P')\<close>
+    by (auto simp: tautology_add_mset)
+  show ?case
+  proof (cases \<open>L \<in># P'\<close>)
+    case True
+    then show ?thesis
+      using mset dist
+      by (metis (no_types, lifting) add_mset_union assms(2) distinct.simps(2) fold_simps(2)
+        insert_DiffM list_update_id mset.simps(2) mset_as_position_nth set_mset_mset
+        sup_union_right1)
+  next
+    case False
+    have [simp]: \<open>length (fold (\<lambda>L xs. xs[atm_of L := Some (is_pos L)]) P xs) = length xs\<close>
+      by (induction P arbitrary: xs) auto
+    moreover have \<open>- L \<notin> set P\<close>
+      using tauto by (metis list.set_intros(1) list.set_intros(2) set_mset_mset tautology_minus)
+    moreover have
+      \<open>fold (\<lambda>L xs. xs[atm_of L := Some (is_pos L)]) P (xs[atm_of L := Some (is_pos L)]) =
+       (fold (\<lambda>L xs. xs[atm_of L := Some (is_pos L)]) P xs) [atm_of L := Some (is_pos L)]\<close>
+      using uL_P dist tauto
+      apply (induction P arbitrary: xs)
+      subgoal by auto
+      subgoal for L' P
+        by (cases \<open>atm_of L = atm_of L'\<close>)
+          (auto simp: tautology_add_mset list_update_swap atm_of_eq_atm_of)
+      done
+    ultimately show ?thesis
+      using mset atm_P_xs dist uL_P False by (auto intro!: mset_as_position.add)
+  qed
+qed
+
+lemma mset_as_position_empty_iff: \<open>mset_as_position xs {#} \<longleftrightarrow> (\<exists>n. xs = replicate n None)\<close>
+  apply (rule iffI)
+  subgoal
+    by (cases rule: mset_as_position.cases, assumption) auto
+  subgoal
+    by (auto intro: mset_as_position.intros)
+  done
+
+type_synonym (in -) lookup_clause_rel = \<open>nat \<times> bool option list\<close>
+
+definition lookup_clause_rel :: \<open>nat multiset \<Rightarrow> (lookup_clause_rel \<times> nat literal multiset) set\<close> where
+\<open>lookup_clause_rel \<A> = {((n, xs), C). n = size C \<and> mset_as_position xs C \<and>
+   (\<forall>L\<in>atms_of (\<L>\<^sub>a\<^sub>l\<^sub>l \<A>). L < length xs)}\<close>
+
+lemma lookup_clause_rel_empty_iff: \<open>((n, xs), C) \<in> lookup_clause_rel \<A> \<Longrightarrow> n = 0 \<longleftrightarrow> C = {#}\<close>
+  by (auto simp: lookup_clause_rel_def)
+
+lemma conflict_atm_le_length: \<open>((n, xs), C) \<in> lookup_clause_rel \<A> \<Longrightarrow> L \<in> atms_of (\<L>\<^sub>a\<^sub>l\<^sub>l \<A>) \<Longrightarrow>
+   L < length xs\<close>
+  by (auto simp: lookup_clause_rel_def)
+
+
+lemma conflict_le_length:
+  assumes
+    c_rel: \<open>((n, xs), C) \<in> lookup_clause_rel \<A>\<close> and
+    L_\<L>\<^sub>a\<^sub>l\<^sub>l: \<open>L \<in># \<L>\<^sub>a\<^sub>l\<^sub>l \<A>\<close>
+  shows \<open>atm_of L < length xs\<close>
+proof -
+  have
+    size: \<open>n = size C\<close> and
+    mset_pos: \<open>mset_as_position xs C\<close> and
+    atms_le: \<open>\<forall>L\<in>atms_of (\<L>\<^sub>a\<^sub>l\<^sub>l \<A>). L < length xs\<close>
+    using c_rel unfolding lookup_clause_rel_def by blast+
+  have \<open>atm_of L \<in> atms_of (\<L>\<^sub>a\<^sub>l\<^sub>l \<A>)\<close>
+    using L_\<L>\<^sub>a\<^sub>l\<^sub>l by (simp add: atms_of_def)
+  then show ?thesis
+    using atms_le by blast
+qed
+
+lemma lookup_clause_rel_atm_in_iff:
+  \<open>((n, xs), C) \<in> lookup_clause_rel \<A> \<Longrightarrow> L \<in># \<L>\<^sub>a\<^sub>l\<^sub>l \<A> \<Longrightarrow> L \<in># C \<longleftrightarrow> xs!(atm_of L) = Some (is_pos L)\<close>
+  by (rule mset_as_position_in_iff_nth)
+     (auto simp: lookup_clause_rel_def atms_of_def)
+
+lemma
+  assumes
+    c: \<open>((n,xs), C) \<in> lookup_clause_rel \<A>\<close>
+  shows
+    lookup_clause_rel_not_tautolgy: \<open>\<not>tautology C\<close> and
+    lookup_clause_rel_distinct_mset: \<open>distinct_mset C\<close> and
+    lookup_clause_rel_size: \<open>isasat_input_bounded \<A> \<Longrightarrow> literals_are_in_\<L>\<^sub>i\<^sub>n \<A> C \<Longrightarrow> size C \<le> 1 + uint32_max div 2\<close>
+proof -
+  have mset: \<open>mset_as_position xs C\<close> and \<open>n = size C\<close> and \<open>\<forall>L\<in>atms_of (\<L>\<^sub>a\<^sub>l\<^sub>l \<A>). L < length xs\<close>
+    using c unfolding lookup_clause_rel_def by fast+
+  show \<open>\<not>tautology C\<close>
+    using mset
+    apply (induction rule: mset_as_position.induct)
+    subgoal by (auto simp: literals_are_in_\<L>\<^sub>i\<^sub>n_def)
+    subgoal by (auto simp: tautology_add_mset)
+    done
+  show \<open>distinct_mset C\<close>
+    using mset mset_as_position_distinct_mset by blast
+  then show \<open>isasat_input_bounded \<A> \<Longrightarrow> literals_are_in_\<L>\<^sub>i\<^sub>n \<A> C \<Longrightarrow> size C \<le> 1 + uint32_max div 2\<close>
+    using simple_clss_size_upper_div2[of \<A> \<open>C\<close>] \<open>\<not>tautology C\<close> by auto
+qed
+
+
+definition option_bool_rel :: \<open>(bool \<times> 'a option) set\<close> where
+  \<open>option_bool_rel = {(b, x). b \<longleftrightarrow> \<not>(is_None x)}\<close>
+
+
+definition NOTIN :: \<open>bool option\<close> where
+  [simp]: \<open>NOTIN = None\<close>
+
+definition ISIN :: \<open>bool \<Rightarrow> bool option\<close> where
+  [simp]: \<open>ISIN b = Some b\<close>
+
+definition is_NOTIN :: \<open>bool option \<Rightarrow> bool\<close> where
+  [simp]: \<open>is_NOTIN x \<longleftrightarrow> x = NOTIN\<close>
+
+lemma is_NOTIN_alt_def:
+  \<open>is_NOTIN x \<longleftrightarrow> is_None x\<close>
+  by (auto split: option.splits)
+
+lemma (in -) mset_as_position_length_not_None:
+   \<open>mset_as_position x2 C \<Longrightarrow> size C = length (filter ((\<noteq>) None) x2)\<close>
+proof (induction rule: mset_as_position.induct)
+  case (empty n)
+  then show ?case by auto
+next
+  case (add xs P L xs') note m_as_p = this(1) and atm_L = this(2)
+  have xs_L: \<open>xs ! (atm_of L) = None\<close>
+  proof -
+    obtain bb :: \<open>bool option \<Rightarrow> bool\<close> where
+      f1: \<open>\<forall>z. z = None \<or> z = Some (bb z)\<close>
+      by (metis option.exhaust)
+    have f2: \<open>xs ! atm_of L \<noteq> Some (is_pos L)\<close>
+      using add.hyps(1) add.hyps(2) add.hyps(3) mset_as_position_in_iff_nth by blast
+    have f3: \<open>\<forall>z b. ((Some b = z \<or> z = None) \<or> bb z) \<or> b\<close>
+      using f1 by blast
+    have f4: \<open>\<forall>zs. (zs ! atm_of L \<noteq> Some (is_pos (- L)) \<or> \<not> atm_of L < length zs)
+           \<or> \<not> mset_as_position zs P\<close>
+      by (metis add.hyps(4) atm_of_uminus mset_as_position_in_iff_nth)
+    have \<open>\<forall>z b. ((Some b = z \<or> z = None) \<or> \<not> bb z) \<or> \<not> b\<close>
+      using f1 by blast
+    then show ?thesis
+      using f4 f3 f2 by (metis add.hyps(1) add.hyps(2) is_pos_neg_not_is_pos)
+  qed
+  obtain xs1 xs2 where
+    xs_xs12: \<open>xs = xs1 @ None # xs2\<close> and
+    xs1: \<open>length xs1 = atm_of L\<close>
+    using atm_L upd_conv_take_nth_drop[of \<open>atm_of L\<close> xs \<open>None\<close>] apply -
+    apply (subst(asm)(2) xs_L[symmetric])
+    by (force simp del: append_take_drop_id)+
+  then show ?case
+    using add by (auto simp: list_update_append)
+qed
+
+
+definition (in -) is_in_lookup_conflict where
+  \<open>is_in_lookup_conflict = (\<lambda>(n, xs) L. \<not>is_None (xs ! atm_of L))\<close>
+
+lemma mset_as_position_remove:
+  \<open>mset_as_position xs D \<Longrightarrow> L < length xs \<Longrightarrow>
+   mset_as_position (xs[L := None]) (remove1_mset (Pos L) (remove1_mset (Neg L) D))\<close>
+proof (induction rule: mset_as_position.induct)
+  case (empty n)
+  then have [simp]: \<open>(replicate n None)[L := None] = replicate n None\<close>
+    using list_update_id[of \<open>replicate n None\<close> L] by auto
+  show ?case by (auto intro: mset_as_position.intros)
+next
+  case (add xs P K xs')
+  show ?case
+  proof (cases \<open>L = atm_of K\<close>)
+    case True
+    then show ?thesis
+      using add by (cases K) auto
+  next
+    case False
+    have map: \<open>mset_as_position (xs[L := None]) (remove1_mset (Pos L) (remove1_mset (Neg L) P))\<close>
+      using add by auto
+    have \<open>K \<notin># P - {#Pos L, Neg L#}\<close> \<open>-K \<notin># P - {#Pos L, Neg L#}\<close>
+      by (auto simp: add.hyps dest!: in_diffD)
+    then show ?thesis
+      using mset_as_position.add[OF map, of \<open>K\<close> \<open>xs[L := None, atm_of K := Some (is_pos K)]\<close>]
+        add False list_update_swap[of \<open>atm_of K\<close> L xs] apply simp
+      apply (subst diff_add_mset_swap)
+      by auto
+  qed
+qed
+
+lemma mset_as_position_remove2:
+  \<open>mset_as_position xs D \<Longrightarrow> atm_of L < length xs \<Longrightarrow>
+   mset_as_position (xs[atm_of L := None]) (D - {#L, -L#})\<close>
+  using mset_as_position_remove[of xs D \<open>atm_of (-L)\<close>]
+  by (smt add_mset_commute add_mset_diff_bothsides atm_of_uminus insert_DiffM
+   literal.exhaust_sel minus_notin_trivial2 remove_1_mset_id_iff_notin uminus_not_id')
+
+definition (in -) delete_from_lookup_conflict
+   :: \<open>nat literal \<Rightarrow> lookup_clause_rel \<Rightarrow> lookup_clause_rel nres\<close> where
+  \<open>delete_from_lookup_conflict = (\<lambda>L (n, xs). do {
+     ASSERT(n\<ge>1);
+     ASSERT(atm_of L < length xs);
+     RETURN (n - 1, xs[atm_of L := None])
+   })\<close>
+
+lemma delete_from_lookup_conflict_op_mset_delete:
+  \<open>(uncurry delete_from_lookup_conflict, uncurry (RETURN oo remove1_mset)) \<in>
+      [\<lambda>(L, D). -L \<notin># D \<and> L \<in># \<L>\<^sub>a\<^sub>l\<^sub>l \<A> \<and> L \<in># D]\<^sub>f Id \<times>\<^sub>f lookup_clause_rel \<A> \<rightarrow>
+      \<langle>lookup_clause_rel \<A>\<rangle>nres_rel\<close>
+  apply (intro frefI nres_relI)
+  subgoal for x y
+    using mset_as_position_remove[of \<open>snd (snd x)\<close> \<open>snd y\<close> \<open>atm_of (fst y)\<close>]
+    apply (cases x; cases y; cases \<open>fst y\<close>)
+    by (auto simp: delete_from_lookup_conflict_def lookup_clause_rel_def
+        dest!: multi_member_split
+        intro!: ASSERT_refine_left)
+  done
+
+definition delete_from_lookup_conflict_pre where
+  \<open>delete_from_lookup_conflict_pre \<A> = (\<lambda>(a, b). - a \<notin># b \<and> a \<in># \<L>\<^sub>a\<^sub>l\<^sub>l \<A> \<and> a \<in># b)\<close>
+
+
+definition add_to_lookup_conflict :: \<open>nat literal \<Rightarrow> lookup_clause_rel \<Rightarrow> lookup_clause_rel\<close> where
+  \<open>add_to_lookup_conflict = (\<lambda>L (n, xs). (if xs ! atm_of L = NOTIN then n + 1 else n,
+      xs[atm_of L := ISIN (is_pos L)]))\<close>
+
+
+
+lemma add_to_lookup_conflict_lookup_clause_rel:
+  assumes
+    confl: \<open>((n, xs), C) \<in> lookup_clause_rel \<A>\<close> and
+    uL_C: \<open>-L \<notin># C\<close> and
+    L_\<L>\<^sub>a\<^sub>l\<^sub>l: \<open>L \<in># \<L>\<^sub>a\<^sub>l\<^sub>l \<A>\<close>
+  shows \<open>(add_to_lookup_conflict L (n, xs), {#L#} \<union># C) \<in> lookup_clause_rel \<A>\<close>
+proof -
+  have
+    n: \<open>n = size C\<close> and
+    mset: \<open>mset_as_position xs C\<close> and
+    atm: \<open>\<forall>L\<in>atms_of (\<L>\<^sub>a\<^sub>l\<^sub>l \<A>). L < length xs\<close>
+    using confl unfolding lookup_clause_rel_def by blast+
+  have \<open>distinct_mset C\<close>
+    using mset by (blast dest: mset_as_position_distinct_mset)
+  have atm_L_xs: \<open>atm_of L < length xs\<close>
+    using atm L_\<L>\<^sub>a\<^sub>l\<^sub>l by (auto simp: atms_of_def)
+  then show ?thesis
+  proof (cases \<open>L \<in># C\<close>)
+    case True
+    with mset have xs: \<open>xs ! atm_of L = Some (is_pos L)\<close> \<open>xs ! atm_of L \<noteq> None\<close>
+      by (auto dest: mset_as_position_nth)
+    moreover have \<open>{#L#} \<union># C = C\<close>
+      using True by (simp add: subset_mset.sup.absorb2)
+    ultimately show ?thesis
+      using n mset atm True
+      by (auto simp: lookup_clause_rel_def add_to_lookup_conflict_def xs[symmetric])
+  next
+    case False
+    with mset have \<open>xs ! atm_of L = None\<close>
+      using mset_as_position_in_iff_nth[of xs C L]
+       mset_as_position_in_iff_nth[of xs C \<open>-L\<close>]  atm_L_xs uL_C
+      by (cases L; cases \<open>xs ! atm_of L\<close>) auto
+    then show ?thesis
+      using n mset atm False atm_L_xs uL_C
+      by (auto simp: lookup_clause_rel_def add_to_lookup_conflict_def
+          intro!: mset_as_position.intros)
+  qed
+qed
+
+
+definition conflict_from_lookup where
+  \<open>conflict_from_lookup = (\<lambda>(n, xs). SPEC(\<lambda>D. mset_as_position xs D \<and> n = size D))\<close>
+
+lemma Ex_mset_as_position:
+  \<open>Ex (mset_as_position xs)\<close>
+proof (induction \<open>size {#x \<in># mset xs. x \<noteq> None#}\<close> arbitrary: xs)
+  case 0
+  then have xs: \<open>xs = replicate (length xs) None\<close>
+    by (auto simp: filter_mset_empty_conv dest: replicate_length_same)
+  show ?case
+    by (subst xs) (auto simp: mset_as_position.empty intro!: exI[of _ \<open>{#}\<close>])
+next
+  case (Suc x) note IH = this(1) and xs = this(2)
+  obtain i where
+     [simp]: \<open>i < length xs\<close> and
+    xs_i: \<open>xs ! i \<noteq> None\<close>
+    using xs[symmetric]
+    by (auto dest!: size_eq_Suc_imp_elem simp: in_set_conv_nth)
+  let ?xs = \<open>xs [i := None]\<close>
+  have \<open>x = size {#x \<in># mset ?xs. x \<noteq> None#}\<close>
+    using xs[symmetric] xs_i by (auto simp: mset_update size_remove1_mset_If)
+  from IH[OF this] obtain D where
+     map: \<open>mset_as_position ?xs D\<close>
+    by blast
+  have [simp]: \<open>Pos i \<notin># D\<close> \<open>Neg i \<notin># D\<close>
+    using xs_i mset_as_position_nth[OF map, of \<open>Pos i\<close>]
+      mset_as_position_nth[OF map, of \<open>Neg i\<close>]
+    by auto
+  have [simp]: \<open>xs ! i = a \<Longrightarrow> xs[i := a] = xs\<close> for a
+    by auto
+
+  have \<open>mset_as_position xs (add_mset (if the (xs ! i) then Pos i else Neg i) D)\<close>
+    using mset_as_position.add[OF map, of \<open>if the (xs ! i) then Pos i else Neg i\<close> xs]
+      xs_i[symmetric]
+    by (cases \<open>xs ! i\<close>) auto
+  then show ?case by blast
+qed
+
+lemma id_conflict_from_lookup:
+  \<open>(RETURN o id, conflict_from_lookup) \<in> [\<lambda>(n, xs). \<exists>D. ((n, xs), D) \<in> lookup_clause_rel \<A>]\<^sub>f Id \<rightarrow>
+    \<langle>lookup_clause_rel \<A>\<rangle>nres_rel\<close>
+  by (intro frefI nres_relI)
+    (auto simp: lookup_clause_rel_def conflict_from_lookup_def RETURN_RES_refine_iff)
+
+
+lemma lookup_clause_rel_exists_le_uint32_max:
+  assumes ocr: \<open>((n, xs), D) \<in> lookup_clause_rel \<A>\<close> and \<open>n > 0\<close> and
+    le_i: \<open>\<forall>k<i. xs ! k = None\<close> and lits: \<open>literals_are_in_\<L>\<^sub>i\<^sub>n \<A> D\<close> and
+    bounded: \<open>isasat_input_bounded \<A>\<close>
+  shows
+    \<open>\<exists>j. j \<ge> i \<and> j < length xs \<and> j < uint32_max \<and> xs ! j \<noteq> None\<close>
+proof -
+  have
+    n_D: \<open>n = size D\<close> and
+    map: \<open>mset_as_position xs D\<close> and
+    le_xs: \<open>\<forall>L\<in>atms_of (\<L>\<^sub>a\<^sub>l\<^sub>l \<A>). L < length xs\<close>
+    using ocr unfolding lookup_clause_rel_def by auto
+  have map_empty: \<open>mset_as_position xs {#} \<longleftrightarrow> (xs = [] \<or> set xs = {None})\<close>
+    by (subst mset_as_position.simps) (auto simp add: list_eq_replicate_iff)
+  have ex_not_none: \<open>\<exists>j. j \<ge> i \<and> j < length xs \<and> xs ! j \<noteq> None\<close>
+  proof (rule ccontr)
+    assume \<open>\<not> ?thesis\<close>
+    then have \<open>xs = [] \<or> set xs = {None}\<close>
+      using le_i by (fastforce simp: in_set_conv_nth)
+    then have \<open>mset_as_position xs {#}\<close>
+      using map_empty by auto
+    then show False
+      using mset_as_position_right_unique[OF map] \<open>n > 0\<close> n_D by (cases D) auto
+  qed
+  then obtain j where
+     j: \<open>j \<ge> i\<close>\<open>j < length xs\<close>\<open>xs ! j \<noteq> None\<close>
+    by blast
+  let ?L = \<open>if the (xs ! j) then Pos j else Neg j\<close>
+  have \<open>?L \<in># D\<close>
+    using j mset_as_position_in_iff_nth[OF map, of ?L] by auto
+  then have \<open>nat_of_lit ?L \<le> uint32_max\<close>
+    using lits bounded
+    by (auto 5 5 dest!: multi_member_split[of _ D]
+        simp: literals_are_in_\<L>\<^sub>i\<^sub>n_add_mset split: if_splits)
+  then have \<open>j < uint32_max\<close>
+    by (auto simp: uint32_max_def split: if_splits)
+  then show ?thesis
+    using j by blast
+qed
+
+definition pre_simplify_clause_inv where
+  \<open>pre_simplify_clause_inv C = (\<lambda>(i, tauto, D, D').
+    i \<le> length C \<and> (\<not>tauto \<longleftrightarrow> \<not>tautology (mset (take i C))) \<and>
+    (\<not>tauto \<longrightarrow> D = remdups_mset (mset (take i C))) \<and>
+    set D' \<subseteq> set C \<and>
+    mset D' = D \<and>
+    \<not>tautology D \<and>
+    distinct_mset D)\<close>
+
+definition pre_simplify_clause :: \<open>'v clause_l \<Rightarrow> (bool \<times> 'v clause_l) nres\<close> where
+  \<open>pre_simplify_clause C = do {
+     (_, tauto, D\<^sub>0, D) \<leftarrow>
+       WHILE\<^sub>T\<^bsup> pre_simplify_clause_inv C\<^esup>
+         (\<lambda>(i, tauto, D, D'). i < length C \<and> \<not>tauto)
+         (\<lambda>(i, tauto, D, D'). do {
+           ASSERT(i < length C);
+           let L = C!i;
+           if -L \<in># D
+           then RETURN (i+1,True, D, D')
+           else if L \<in># D
+           then RETURN (i+1, tauto, D, D')
+           else RETURN (i+1,tauto, add_mset L D, D' @ [L])
+         })
+         (0, False, {#}, []);
+     ASSERT(D\<^sub>0 = mset D \<and> set D \<subseteq> set C);
+     RETURN (tauto, D)
+  }\<close>
+
+definition pre_simplify_clause_spec where
+  \<open>pre_simplify_clause_spec C = (\<lambda>(tauto, D).
+    (tauto \<longleftrightarrow> tautology (mset C)) \<and>
+    (\<not>tauto \<longrightarrow> mset D = remdups_mset (mset C)))\<close>
+
+lemma pre_simplify_clause_spec:
+  \<open>pre_simplify_clause C \<le>  \<Down> Id (SPEC(pre_simplify_clause_spec C))\<close>
+proof -
+  have [refine0]: \<open>wf (measure (\<lambda>(i, _). length C - i))\<close>
+    by auto
+  show ?thesis
+    unfolding pre_simplify_clause_def
+    apply refine_vcg
+    subgoal by (auto simp: pre_simplify_clause_inv_def)
+    subgoal by auto
+    subgoal for state i b tauto ba D D'
+      by (auto simp: pre_simplify_clause_inv_def
+        take_Suc_conv_app_nth tautology_add_mset)
+    subgoal
+      by auto
+    subgoal for state i b tauto ba D D'
+      by (auto simp: pre_simplify_clause_inv_def
+        take_Suc_conv_app_nth tautology_add_mset)
+    subgoal
+      by auto
+    subgoal for state i b tauto ba D D'
+      by (auto simp: pre_simplify_clause_inv_def
+        take_Suc_conv_app_nth tautology_add_mset)
+    subgoal
+      by auto
+    subgoal by (auto simp: pre_simplify_clause_inv_def)
+    subgoal by (auto simp: pre_simplify_clause_inv_def)
+    subgoal for state i b tauto ba D D'
+      using not_tautology_mono[of \<open>mset (take i C)\<close> \<open>mset C\<close>]
+      by (auto simp: pre_simplify_clause_inv_def mset_take_subseteq
+        pre_simplify_clause_spec_def)
+    done
+qed
+
+definition (in -) lit_is_in_lookup where
+  \<open>lit_is_in_lookup = (\<lambda>L (n, xs). do {
+     ASSERT(atm_of L < length xs);
+     RETURN ((xs ! atm_of L) = Some (is_pos L))})\<close>
+
+definition unmark_clause :: \<open>_\<close> where
+  \<open>unmark_clause C lup = do {
+     (_, lup) \<leftarrow> WHILE\<^sub>T
+       (\<lambda>(i,lup). i < length C)
+        (\<lambda>(i,lup).  do {
+          ASSERT(i < length C);
+          lup \<leftarrow> delete_from_lookup_conflict (C!i) lup;
+          RETURN (i+1, lup)
+       })
+       (0, lup);
+     RETURN lup
+  }\<close>
+
+lemma unmark_clause_spec:
+  assumes \<open>(lup, mset C) \<in> lookup_clause_rel \<A>\<close> \<open>atm_of ` set C \<subseteq> set_mset \<A>\<close>
+  shows \<open>unmark_clause C lup \<le> (SPEC(\<lambda>lup'. (lup', {#}) \<in> lookup_clause_rel \<A>))\<close>
+proof -
+  have [refine]: \<open>wf (measure (\<lambda>(i, _). length C - i))\<close>
+    by auto
+  show ?thesis
+    unfolding unmark_clause_def
+    apply (refine_vcg WHILET_rule[where R = \<open>measure (\<lambda>(i, _). length C - i)\<close> and
+      I = \<open>\<lambda>(i,lup). (lup, mset (drop i C)) \<in> lookup_clause_rel \<A>\<close>])
+    subgoal using assms by auto
+    subgoal using assms by auto
+    subgoal for s a b
+      using lookup_clause_rel_not_tautolgy[of \<open>fst b\<close> \<open>snd b\<close> \<open>mset (drop a C)\<close>] assms(2) apply -
+      apply (rule 
+        delete_from_lookup_conflict_op_mset_delete[of \<A>, THEN fref_to_Down_curry,
+          of \<open>C!a\<close> \<open>mset (drop a C)\<close>, THEN order_trans])
+      by (auto simp: in_\<L>\<^sub>a\<^sub>l\<^sub>l_atm_of_\<A>\<^sub>i\<^sub>n conc_fun_RES RETURN_def tautology_add_mset
+        simp flip: Cons_nth_drop_Suc)
+    subgoal
+      by auto
+    done
+qed
+
+lemma lit_is_in_lookup_spec:
+  assumes \<open>(lup, C) \<in> lookup_clause_rel \<A>\<close> \<open>atm_of L \<in># \<A>\<close>
+  shows \<open>lit_is_in_lookup L lup = RES {L \<in># C}\<close>
+  using assms unfolding lit_is_in_lookup_def
+  apply refine_rcg
+  using mset_as_position_in_iff_nth[of \<open>snd lup\<close> C L]
+  by (auto simp: lit_is_in_lookup_def lookup_clause_rel_def atms_of_\<L>\<^sub>a\<^sub>l\<^sub>l_\<A>\<^sub>i\<^sub>n
+    dest: multi_member_split
+    dest: mset_as_position_nth)
+
+definition pre_simplify_clause_lookup
+  :: \<open>nat clause_l \<Rightarrow> lookup_clause_rel \<Rightarrow>(bool \<times> nat clause_l \<times> lookup_clause_rel) nres\<close>
+  where
+  \<open>pre_simplify_clause_lookup C lup = do {
+  (_, tauto, lup, D) \<leftarrow>
+  WHILE\<^sub>T\<^bsup> \<lambda>_. True\<^esup>
+    (\<lambda>(i, tauto, D, D'). i < length C \<and> \<not>tauto)
+    (\<lambda>(i, tauto, D, D'). do {
+      ASSERT(i < length C);
+      ASSERT(fst D < uint32_max \<and> atm_of (C!i) < length (snd D));
+      ASSERT(length D' = fst D);
+      let L = C!i;
+      b \<leftarrow> lit_is_in_lookup (-L) D;
+      if b
+      then RETURN (i+1,True, D, D')
+      else do {
+        b \<leftarrow> lit_is_in_lookup L D;
+        if b
+        then RETURN (i+1, tauto, D, D')
+        else RETURN (i+1,tauto, add_to_lookup_conflict L D, D' @ [L])
+      }
+    })
+    (0, False, lup, []);
+  lup \<leftarrow> unmark_clause D lup;
+  RETURN (tauto, D, lup)
+}\<close>
+
+lemma pre_simplify_clause_lookup_pre_simplify_clause:
+  assumes \<open>(lup, {#}) \<in> lookup_clause_rel \<A>\<close> \<open>atm_of ` set C \<subseteq> set_mset \<A>\<close> \<open>isasat_input_bounded \<A>\<close>
+  shows \<open>pre_simplify_clause_lookup C lup \<le>
+    \<Down>{((tauto, D, lup), (tauto', D')). tauto=tauto' \<and> D=D' \<and> (lup, {#}) \<in> lookup_clause_rel \<A>}
+      (pre_simplify_clause C)\<close>
+proof -
+  have [refine0]: \<open>((0, False, lup, []), 0, False, {#}, []) \<in>
+     nat_rel \<times>\<^sub>r bool_rel \<times>\<^sub>r lookup_clause_rel \<A> \<times>\<^sub>r \<langle>Id\<rangle>list_rel\<close>
+    using assms by auto
+  have [simp]: \<open>x < length C \<Longrightarrow> atm_of (- C ! x) \<in># \<A>\<close>
+    \<open>x < length C \<Longrightarrow> atm_of (C ! x) \<in># \<A>\<close> for x
+    using assms by auto
+  show ?thesis
+    using assms
+    unfolding pre_simplify_clause_lookup_def pre_simplify_clause_def
+    apply (refine_vcg lit_is_in_lookup_spec lhs_step_If)
+    subgoal by auto
+    subgoal by auto
+    subgoal by auto
+    subgoal for x x' x1 x2 x1a x2a x1b x2b x1c x2c x1d x2d x1e x2e
+      using simple_clss_size_upper_div2[of \<A> \<open>mset x2b\<close>] assms
+      unfolding  literals_are_in_\<L>\<^sub>i\<^sub>n_alt_def apply -
+      by (subgoal_tac \<open>atm_of ` set (take x1 C) \<subseteq> atms_of (\<L>\<^sub>a\<^sub>l\<^sub>l \<A>)\<close>)   
+        (auto simp: lit_is_in_lookup_spec in_\<L>\<^sub>a\<^sub>l\<^sub>l_atm_of_\<A>\<^sub>i\<^sub>n pre_simplify_clause_inv_def
+        lookup_clause_rel_def uint32_max_def atms_of_\<L>\<^sub>a\<^sub>l\<^sub>l_\<A>\<^sub>i\<^sub>n dest!: in_set_takeD)
+    subgoal for x x' x1 x2 x1a x2a x1b x2b x1c x2c x1d x2d x1e x2e
+      using simple_clss_size_upper_div2[of \<A> \<open>mset x2b\<close>] assms
+      unfolding  literals_are_in_\<L>\<^sub>i\<^sub>n_alt_def apply -
+      by (subgoal_tac \<open>atm_of ` set (take x1 C) \<subseteq> atms_of (\<L>\<^sub>a\<^sub>l\<^sub>l \<A>)\<close>)   
+        (auto simp: lit_is_in_lookup_spec in_\<L>\<^sub>a\<^sub>l\<^sub>l_atm_of_\<A>\<^sub>i\<^sub>n pre_simplify_clause_inv_def
+        lookup_clause_rel_def uint32_max_def atms_of_\<L>\<^sub>a\<^sub>l\<^sub>l_\<A>\<^sub>i\<^sub>n dest!: in_set_takeD)
+    subgoal by (clarsimp simp add: lookup_clause_rel_def pre_simplify_clause_inv_def
+      simp del: size_mset simp flip: size_mset)
+    subgoal for x x' x1 x2 x1a x2a x1b x2b x1c x2c x1d x2d x1e x2e
+      using add_to_lookup_conflict_lookup_clause_rel[of \<open>fst x1e\<close> \<open>snd x1e\<close> x1b \<A> \<open>C ! x1\<close>]
+      by (auto simp: lit_is_in_lookup_spec in_\<L>\<^sub>a\<^sub>l\<^sub>l_atm_of_\<A>\<^sub>i\<^sub>n)
+    subgoal for x x' x1 x2 x1a x2a x1b x2b x1c x2c x1d x2d x1e x2e
+      by (rule unmark_clause_spec[of _ _ \<A>, THEN order_trans])
+        auto
+    done
+qed
+
+end
