Weidenbach_Book/IsaSAT/IsaSAT_Mark_LLVM.thy
@@ -1,0 +1,110 @@
+theory IsaSAT_Mark_LLVM
+  imports IsaSAT_Mark
+    IsaSAT_Literals_LLVM
+begin
+
+type_synonym mark = \<open>bool option\<close>
+
+definition mark_rel_aux :: \<open>(int \<times> mark) set\<close> where
+  \<open>mark_rel_aux = {(0, None), (1, Some True), (-1, Some False)}\<close>
+
+definition mark_rel :: \<open>(3 word \<times> bool option) set\<close> where
+  \<open>mark_rel = sint_rel' TYPE(3) O mark_rel_aux\<close>
+
+abbreviation mark_assn :: \<open>mark \<Rightarrow> 3 word \<Rightarrow> assn\<close> where
+  \<open>mark_assn \<equiv> pure mark_rel\<close>
+
+definition marked_struct_rel :: \<open>(_ \<times> lookup_clause_rel) set\<close> where
+  \<open>marked_struct_rel = Id \<times>\<^sub>r \<langle>mark_rel_aux\<rangle>list_rel\<close>
+
+definition marked_struct_assn :: \<open>lookup_clause_rel \<Rightarrow> _ \<Rightarrow> assn\<close> where
+  \<open>marked_struct_assn = uint32_nat_assn \<times>\<^sub>a array_assn (pure mark_rel)\<close>
+
+definition Mark :: \<open>bool \<Rightarrow> bool option\<close> where [simp]: \<open>Mark = Some\<close>
+definition NoMark :: \<open>bool option\<close> where [simp]: \<open>NoMark = None\<close>
+
+lemmas mark_defs = Mark_def[symmetric] NoMark_def[symmetric]
+
+lemmas [fcomp_norm_unfold] = mark_rel_aux_def[symmetric] mark_rel_def[symmetric]
+
+sepref_def Mark_impl [llvm_inline]
+  is [] \<open>RETURN o (\<lambda>b. if b then 1 else -1)\<close> :: \<open>bool1_assn\<^sup>k \<rightarrow>\<^sub>a sint_assn' TYPE(3)\<close>
+  apply (annot_sint_const \<open>TYPE(3)\<close>)
+  by sepref
+
+sepref_def NoMark_impl [llvm_inline]
+  is [] \<open>uncurry0 (RETURN 0)\<close> :: \<open>unit_assn\<^sup>k \<rightarrow>\<^sub>a sint_assn' TYPE(3)\<close>
+  apply (annot_sint_const \<open>TYPE(3)\<close>)
+  by sepref
+
+sepref_register Mark NoMark
+
+lemma Mark_rel_aux: \<open>(\<lambda>b. if b then 1 :: int else -1, Mark) \<in> bool_rel \<rightarrow> mark_rel_aux\<close>
+  by (auto intro: frefI split: if_splits simp: mark_rel_aux_def)
+
+lemmas [sepref_fr_rules] =
+  Mark_impl.refine[FCOMP Mark_rel_aux]
+
+lemma NoMark_rel_aux: \<open>(0, NoMark) \<in> mark_rel_aux\<close>
+  by (auto intro: frefI split: if_splits simp: mark_rel_aux_def)
+
+lemmas [sepref_fr_rules] =
+  NoMark_impl.refine[FCOMP NoMark_rel_aux]
+
+lemma mark_rel_aux_eq:  \<open>((=), (=)) \<in> mark_rel_aux \<rightarrow> mark_rel_aux \<rightarrow> bool_rel\<close>
+  by (auto intro!: frefI simp: mark_rel_aux_def)
+
+sepref_def mark_eq_impl is
+  \<open>uncurry (RETURN oo (=))\<close> :: \<open>(sint_assn' TYPE(3))\<^sup>d *\<^sub>a (sint_assn' TYPE(3))\<^sup>d \<rightarrow>\<^sub>a bool1_assn\<close>
+  unfolding mark_rel_aux_def
+  by sepref
+
+lemmas [sepref_fr_rules] = mark_eq_impl.refine[FCOMP mark_rel_aux_eq]
+
+sepref_register \<open>(=) :: mark \<Rightarrow> _ \<Rightarrow> _\<close> lit_is_in_lookup delete_from_lookup_conflict unmark_clause
+  add_to_lookup_conflict pre_simplify_clause_lookup
+
+sepref_def lit_is_in_lookup_impl
+  is \<open>uncurry lit_is_in_lookup\<close>
+  :: \<open>unat_lit_assn\<^sup>k *\<^sub>a marked_struct_assn\<^sup>k \<rightarrow>\<^sub>a bool1_assn\<close>
+  unfolding lit_is_in_lookup_def mark_defs marked_struct_assn_def
+    array_fold_custom_replicate
+  apply (annot_all_atm_idxs)
+  by sepref
+
+sepref_def delete_from_lookup_conflict_impl
+  is \<open>uncurry delete_from_lookup_conflict\<close>
+  :: \<open>unat_lit_assn\<^sup>k *\<^sub>a marked_struct_assn\<^sup>d \<rightarrow>\<^sub>a marked_struct_assn\<close>
+  unfolding delete_from_lookup_conflict_def mark_defs marked_struct_assn_def
+  apply (annot_unat_const \<open>TYPE(32)\<close>)
+  apply (annot_all_atm_idxs)
+  by sepref
+abbreviation clause_ll_assn where
+  \<open>clause_ll_assn \<equiv> al_assn' TYPE(64) unat_lit_assn\<close>
+
+sepref_def unmark_clause_impl
+  is \<open>uncurry unmark_clause\<close>
+  :: \<open>clause_ll_assn\<^sup>k *\<^sub>a marked_struct_assn\<^sup>d \<rightarrow>\<^sub>a marked_struct_assn\<close>
+  unfolding unmark_clause_def
+  apply (annot_snat_const \<open>TYPE(64)\<close>)
+  by sepref
+
+sepref_def add_to_lookup_conflict
+  is \<open>uncurry (RETURN oo add_to_lookup_conflict)\<close>
+  :: \<open>[\<lambda>(L, n, D). atm_of L < length D \<and> n < uint32_max]\<^sub>a
+    unat_lit_assn\<^sup>k *\<^sub>a marked_struct_assn\<^sup>d \<rightarrow> marked_struct_assn\<close>
+  unfolding mark_defs marked_struct_assn_def add_to_lookup_conflict_def NOTIN_def ISIN_def
+  apply (annot_unat_const \<open>TYPE(32)\<close>)
+  apply (annot_all_atm_idxs)
+  by sepref
+
+sepref_def pre_simplify_clause_lookup_impl
+  is \<open>uncurry pre_simplify_clause_lookup\<close>
+  :: \<open>clause_ll_assn\<^sup>k *\<^sub>a marked_struct_assn\<^sup>d \<rightarrow>\<^sub>a bool1_assn \<times>\<^sub>a clause_ll_assn \<times>\<^sub>a marked_struct_assn\<close>
+  unfolding pre_simplify_clause_lookup_def
+  apply (rewrite at \<open>(_, _, _, \<hole>)\<close> al_fold_custom_empty[where 'l=64])
+  supply [[goals_limit=1]]
+  apply (annot_snat_const \<open>TYPE(64)\<close>)
+  by sepref
+
+end
